CardanoLedgerApi/V3/Governance.lean
@@ -1,4 +1,6 @@
 import CardanoLedgerApi.IsData.Class
+import CardanoLedgerApi.V1
+import CardanoLedgerApi.V2
 import CardanoLedgerApi.V3.Tx
 import CardanoLedgerApi.V3.TxCert
 import PlutusCore
@@ -13,15 +15,9 @@ namespace V3
   )
 end V3
 
-namespace V2
-  open CardanoLedgerApi.V2
-  export CardanoLedgerApi.V2 (
-    PubKeyHash
-  )
-end V2
-
 open IsData.Class
 open TxCert (ColdCommitteeCredential DRepCredential HotCommitteeCredential)
+open CardanoLedgerApi.Extras (Option_lt_irrefl)
 open PlutusCore.Data (Data)
 open PlutusCore.Integer (Integer)
 
@@ -316,13 +312,275 @@ instance : IsData GovernanceActionId where
   | _ => none
 
 
+structure ProtocolVersion where
+  pvMajor : Integer
+  pvMinor : Integer
+deriving Repr
+
+def beqProtocolVersion (x y : ProtocolVersion) : Bool :=
+  x.pvMajor == y.pvMajor &&
+  x.pvMinor == y.pvMinor
+
+/-- BEq instance for ProtocolVersion -/
+instance : BEq ProtocolVersion := ⟨beqProtocolVersion⟩
+
+/-! DecidableEq instance for ProtocolVersion -/
+@[simp] theorem beqProtocolVersion_iff_eq (x y : ProtocolVersion) : beqProtocolVersion x y ↔ x = y := by
+  cases x <;> cases y <;> simp [beqProtocolVersion]
+
+@[simp] theorem beqProtocolVersion_false_iff_not_eq (x y : ProtocolVersion) : beqProtocolVersion x y = false ↔ x ≠ y := by
+  cases x <;> cases y <;> simp [beqProtocolVersion]
+
+def decEqProtocolVersion (x y : ProtocolVersion) : Decidable (Eq x y) :=
+  match h:(beqProtocolVersion x y) with
+  | true => isTrue ((beqProtocolVersion_iff_eq _ _).1 h)
+  | false => isFalse ((beqProtocolVersion_false_iff_not_eq _ _).1 h)
+
+instance : DecidableEq ProtocolVersion := decEqProtocolVersion
+
+/-! LawfulBEq instance for ProtocolVersion -/
+theorem beqProtocolVersion_reflexive (x : ProtocolVersion) : beqProtocolVersion x x = true := by
+   cases x <;> simp [beqProtocolVersion]
+
+instance : LawfulBEq ProtocolVersion where
+  eq_of_beq {a b} := (beqProtocolVersion_iff_eq a b).1
+  rfl {bs} := by simp [BEq.beq]
+
+def ltProtocolVersion (x y : ProtocolVersion) : Bool :=
+  x.pvMajor < y.pvMajor || (x.pvMajor = y.pvMajor && x.pvMinor < y.pvMinor)
+
+/-- LT instance for ProtocolVersion -/
+instance : LT ProtocolVersion where
+  lt x y := ltProtocolVersion x y
+
+/-! DecidableLT instance for ProtocolVersion -/
+theorem ltProtocolVersion_true_imp_lt (x y : ProtocolVersion) : ltProtocolVersion x y → x < y := by
+  cases x <;> cases y <;> simp only [ltProtocolVersion, LT.lt] <;> simp
+
+theorem ltProtocolVersion_false_imp_not_lt (x y : ProtocolVersion) :
+  ltProtocolVersion x y = false → ¬ x < y := by
+    cases x <;> cases y <;> simp only [ltProtocolVersion, LT.lt] <;> simp
+
+def decLtProtocolVersion (x y : ProtocolVersion) : Decidable (LT.lt x y) :=
+  match h:(ltProtocolVersion x y) with
+  | true => isTrue (ltProtocolVersion_true_imp_lt _ _ h)
+  | false => isFalse (ltProtocolVersion_false_imp_not_lt _ _ h)
+
+instance : DecidableLT ProtocolVersion := decLtProtocolVersion
+
+/-! Std.Irrefl instance for ProtocolVersion -/
+@[simp] theorem ltProtocolVersion_same_false (x : ProtocolVersion) : ltProtocolVersion x x = false :=
+  by cases x <;> simp [ltProtocolVersion]
+
+@[simp] theorem ProtocolVersion_lt_irrefl (x : ProtocolVersion) : ¬ x < x := by cases x <;> simp [LT.lt]
+
+instance : Std.Irrefl (. < . : ProtocolVersion → ProtocolVersion → Prop) where
+  irrefl := ProtocolVersion_lt_irrefl
+
+/-- LE instance for ProtocolVersion -/
+instance : LE ProtocolVersion where
+  le x y := ¬ (y < x)
+
+/-! DecidableLE instance for ProtocolVersion -/
+instance : DecidableLE ProtocolVersion :=
+  fun x y => inferInstanceAs (Decidable (¬ (y < x)))
+
+
+/-- IsData instance for ProtocolVersion -/
+instance : IsData ProtocolVersion where
+  toData x := mkDataConstr 0 [Data.I x.pvMajor, Data.I x.pvMinor]
+  fromData
+  | Data.Constr 0 [Data.I maj, Data.I min] => some ⟨maj, min⟩
+  | _ => none
+
+
+/-- A Plutus Data object containing proposed parameter changes. The Data object contains
+a @Map@ with one entry per changed parameter, from the parameter ID to the new value.
+Unchanged parameters are not included.
+
+The mapping from parameter IDs to parameters can be found in
+[conway.cddl](https://github.com/IntersectMBO/cardano-ledger/blob/master/eras/conway/impl/cddl-files/conway.cddl).
+
+/Invariant:/ This map is non-empty, and the keys are stored in ascending order.
+
+-/
+abbrev ChangedParameters := Data
+
+abbrev Withdrawals := List (V2.Credential × Integer) -- handled as a Data.Map at the Data level
+
+/-- Return the list `Data × Data` representation for Withdrawals. -/
+def withdrawalsToListPairData (xs : Withdrawals) : List (Data × Data) :=
+  Recursor.map x in xs with (IsData.toData x.1, Data.I x.2)
+
+/-- Try to decode `Withdrawals` from a `Data × Data` list instance. -/
+def listPairDataToWithdrawals (xs : List (Data × Data)) : Option Withdrawals :=
+  match xs with
+  | [] => some []
+  | (d1, Data.I i) :: xs' =>
+      match IsData.fromData d1, listPairDataToWithdrawals xs' with
+      | some cred, some rest => (cred, i) :: rest
+      | _, _ => none
+  | _ => none
+
+/-- IsData instance for Withdrawals -/
+instance : IsData Withdrawals where
+  toData x := Data.Map (withdrawalsToListPairData x)
+  fromData
+  | Data.Map r_wdrwl => listPairDataToWithdrawals r_wdrwl
+  | _ => none
+
+abbrev NewCommitteeMembers := List (ColdCommitteeCredential × Integer) -- handled as Data.Map at Data level
+
+/-- Return the list `Data × Data` representation for NewCommitteeMembers. -/
+def newCommitteeToListPairData (xs : NewCommitteeMembers) : List (Data × Data) :=
+  Recursor.map x in xs with (IsData.toData x.1, Data.I x.2)
+
+/-- Try to decode `NewCommitteeMembers` from a `Data × Data` list instance. -/
+def listPairDataToNewCommittee (xs : List (Data × Data)) : Option NewCommitteeMembers :=
+  match xs with
+  | [] => some []
+  | (d1, Data.I i) :: xs' =>
+      match IsData.fromData d1, listPairDataToNewCommittee xs' with
+      | some cred, some rest => (cred, i) :: rest
+      | _, _ => none
+  | _ => none
+
+/-- IsData instance for NewCommitteemembers -/
+instance : IsData NewCommitteeMembers where
+  toData x := Data.Map (newCommitteeToListPairData x)
+  fromData
+  | Data.Map r_cm => listPairDataToNewCommittee r_cm
+  | _ => none
+
+
+/-- Rational kept at Data level -/
+abbrev Quorum := Data
+
+/-- A constitution. The optional anchor is omitted. -/
+abbrev Constitution := Option V2.ScriptHash
+
+abbrev OldCommitteeMembers := List ColdCommitteeCredential
+
+/-- Return the list `Data` representation for a `OldCommitteeMembers`. -/
+def oldCommitteeToListData (xs : OldCommitteeMembers) : List Data :=
+  Recursor.map x in xs with IsData.toData x
+
+/-- Try to decode `OldCommitteeMembers` from a `Data` list instance. -/
+def listDataToOldCommittee (xs : List Data) : Option OldCommitteeMembers :=
+  match xs with
+  | [] => some []
+  | d :: xs' =>
+      match IsData.fromData d, listDataToOldCommittee xs' with
+      | some cred, some rest => cred :: rest
+      | _, _ => none
+
+/-- IsData instance for OldCommitteeMembers -/
+instance : IsData OldCommitteeMembers where
+  toData x := Data.List (oldCommitteeToListData x)
+  fromData
+  | Data.List r_cm => listDataToOldCommittee r_cm
+  | _ => none
+
+
+/-- A governance action. -/
+inductive GovernanceAction where
+ /-- Hash of the constitution script -/
+ | ParameterChange : Option GovernanceActionId → ChangedParameters → Option V2.ScriptHash → GovernanceAction
+ /-- Proposal to update protocol version -/
+ | HardForkInitiation : Option GovernanceActionId → ProtocolVersion → GovernanceAction
+ /-- Hash of the constitution script -/
+ | TreasuryWithdrawals : Withdrawals → Option V2.ScriptHash → GovernanceAction
+ | NoConfidence : Option GovernanceActionId → GovernanceAction
+ | UpdateCommittee : Option GovernanceActionId → OldCommitteeMembers → NewCommitteeMembers → Quorum → GovernanceAction
+ | NewConstitution : Option GovernanceActionId → Constitution → GovernanceAction
+ | InfoAction
+deriving Repr
+
+
+def beqGovernanceAction (x y : GovernanceAction) : Bool :=
+  match x, y with
+  | .ParameterChange a c s, .ParameterChange a' c' s' => a == a' && c == c' && s == s'
+  | .HardForkInitiation a p, .HardForkInitiation a' p' => a == a' && p == p'
+  | .TreasuryWithdrawals w s, .TreasuryWithdrawals w' s' => w == w' && s == s'
+  | .NoConfidence a, .NoConfidence a' => a == a'
+  | .UpdateCommittee a old new q, .UpdateCommittee a' old' new' q' => a == a' && old == old' && new == new' && q == q'
+  | .NewConstitution a c, .NewConstitution a' c' => a == a' && c == c'
+  | .InfoAction, .InfoAction => true
+  | _, _ => false
+
+/-- BEq instance for Voter -/
+instance : BEq GovernanceAction := ⟨beqGovernanceAction⟩
+
+/-! DecidableEq instance for GovernanceAction -/
+@[simp] theorem beqGovernanceAction_iff_eq (x y : GovernanceAction) : beqGovernanceAction x y ↔ x = y := by
+  cases x <;> cases y <;> simp [beqGovernanceAction] <;>
+  apply Iff.intro <;>
+    . repeat' rw [and_imp];
+      intros; repeat' constructor <;> repeat' assumption
+
+@[simp] theorem beqGovernanceAction_false_iff_not_eq (x y : GovernanceAction) : beqGovernanceAction x y = false ↔ x ≠ y := by
+  cases x <;> cases y <;> simp [beqGovernanceAction]
+
+def decEqGovernanceAction (x y : GovernanceAction) : Decidable (Eq x y) :=
+  match h:(beqGovernanceAction x y) with
+  | true => isTrue ((beqGovernanceAction_iff_eq _ _).1 h)
+  | false => isFalse ((beqGovernanceAction_false_iff_not_eq _ _).1 h)
+
+instance : DecidableEq GovernanceAction := decEqGovernanceAction
+
+/-! LawfulBEq instance for GovernanceAction -/
+theorem beqGovernanceAction_reflexive (x : GovernanceAction) : beqGovernanceAction x x = true := by
+   cases x <;> simp [beqGovernanceAction]
+
+instance : LawfulBEq GovernanceAction where
+  eq_of_beq {a b} := (beqGovernanceAction_iff_eq a b).1
+  rfl {bs} := by simp [BEq.beq]
+
+/-- IsData instance for GovernanceAction -/
+instance : IsData GovernanceAction where
+  toData
+  | .ParameterChange a c s => mkDataConstr 0 [IsData.toData a, IsData.toData c, IsData.toData s]
+  | .HardForkInitiation a p => mkDataConstr 1 [IsData.toData a, IsData.toData p]
+  | .TreasuryWithdrawals w s => mkDataConstr 2 [IsData.toData w, IsData.toData s]
+  | .NoConfidence a => mkDataConstr 3 [IsData.toData a]
+  | .UpdateCommittee a old new q => mkDataConstr 4 [IsData.toData a, IsData.toData old, IsData.toData new, IsData.toData q]
+  | .NewConstitution a c => mkDataConstr 5 [IsData.toData a, IsData.toData c]
+  | .InfoAction => mkDataConstr 6
+  fromData
+  | Data.Constr 0 [r_a, r_c, r_s] =>
+        match IsData.fromData r_a, IsData.fromData r_c, IsData.fromData r_s with
+        | some a, some c, some s => some (.ParameterChange a c s)
+        | _, _, _ => none
+  | Data.Constr 1 [r_a, r_p] =>
+        match IsData.fromData r_a, IsData.fromData r_p with
+        | some a, some p => some (.HardForkInitiation a p)
+        | _, _ => none
+  | Data.Constr 2 [r_w, r_s] =>
+        match IsData.fromData r_w, IsData.fromData r_s with
+        | some w, some s => some (.TreasuryWithdrawals w s)
+        | _, _ => none
+  | Data.Constr 3 [r_a] =>
+        match IsData.fromData r_a with
+        | some a => some (.NoConfidence a)
+        | none => none
+  | Data.Constr 4 [r_a, r_old, r_new, q] =>
+        match IsData.fromData r_a, IsData.fromData r_old, IsData.fromData r_new with
+        | some a, some old, some new => some (.UpdateCommittee a old new q)
+        | _, _, _ => none
+  | Data.Constr 5 [r_a, r_c] =>
+        match IsData.fromData r_a, IsData.fromData r_c with
+        | some a, some c => some (.NewConstitution a c)
+        | _, _ => none
+  | Data.Constr 6 [] => some .InfoAction
+  | _ => none
+
+
 /-- A proposal procedure. The optional anchor is omitted. -/
 structure ProposalProcedure where
   ppDeposit : Integer
   ppReturnAddr : V2.Credential
   ppGovernanceAction : Data -- keep at Data level
 deriving Repr
-
 
 def beqProposalProcedure (x y : ProposalProcedure) : Bool :=
   x.ppDeposit == y.ppDeposit &&
@@ -405,9 +663,9 @@ instance : DecidableLE ProposalProcedure :=
 instance : IsData ProposalProcedure where
   toData x := mkDataConstr 0 [IsData.toData x.ppDeposit, IsData.toData x.ppReturnAddr, x.ppGovernanceAction]
   fromData
-  | Data.Constr 0 [r_deposit, r_addr, action] =>
+  | Data.Constr 0 [r_deposit, r_addr, r_action] =>
       match IsData.fromData r_deposit, IsData.fromData r_addr with
-      | some deposit, some addr => some ⟨deposit, addr, action⟩
+      | some deposit, some addr => some ⟨deposit, addr, r_action⟩
       | _, _ => none
   | _ => none
 
