CardanoLedgerApi/Extras.lean
@@ -1,0 +1,55 @@
+
+namespace CardanoLedgerApi.Extras
+
+def ltOption [LT α] [DecidableLT α] (x y : Option α) : Bool :=
+  match x, y with
+  | .none, .some _ => true
+  | .some a, .some b => a < b
+  | _, _ => false
+
+/-! DecidableLT instance for Option -/
+theorem ltOption_true_imp_lt [LT α] [DecidableLT α] (x y : Option α) : ltOption x y → x < y := by
+  cases x <;> cases y <;> simp [ltOption, LT.lt, Option.lt]
+
+theorem ltOption_false_imp_not_lt [LT α] [DecidableLT α] (x y : Option α) : ltOption x y = false → ¬ x < y := by
+  cases x <;> cases y <;> simp [ltOption, LT.lt, Option.lt]
+
+def decLtOption [LT α] [DecidableLT α] (x y : Option α) : Decidable (LT.lt x y) :=
+  match h:(ltOption x y) with
+  | true => isTrue (ltOption_true_imp_lt _ _ h)
+  | false => isFalse (ltOption_false_imp_not_lt _ _ h)
+
+instance [LT α] [DecidableLT α] : DecidableLT (Option α) := decLtOption
+
+/-- LE instance for Option -/
+instance [LT α] : LE (Option α) where
+  le x y := ¬ (y < x)
+
+def leqOption [LT α] [DecidableLT α] (x y : Option α) : Bool := !(y < x)
+
+/-! DecidableLE instance for Option -/
+theorem leqOption_true_imp_le [LT α] [DecidableLT α] (x y : Option α) : leqOption x y → x ≤ y := by
+  cases x <;> cases y <;> simp [leqOption, LE.le]
+
+theorem leqOption_false_imp_not_le [LT α] [DecidableLT α] (x y : Option α) : leqOption x y = false → ¬ x ≤ y := by
+  cases x <;> cases y <;> simp [leqOption, LE.le]
+
+def decLeqOption [LT α] [DecidableLT α] (x y : Option α) : Decidable (LE.le x y) :=
+  match h:(leqOption x y) with
+  | true => isTrue (leqOption_true_imp_le _ _ h)
+  | false => isFalse (leqOption_false_imp_not_le _ _ h)
+
+instance [LT α] [DecidableLT α] : DecidableLE (Option α) := decLeqOption
+
+/-! Std.Irrefl instance for Option -/
+@[simp] theorem ltOptionD_same_false [LT α] [DecidableLT α] [Std.Irrefl (. < . : α → α → Prop)] (x : Option α) :
+  ltOption x x = false := by cases x <;> simp [ltOption, Std.Irrefl.irrefl]
+
+theorem Option_lt_irrefl [LT α] [DecidableLT α] [Std.Irrefl (. < . : α → α → Prop)] (x : Option α) : ¬ x < x :=
+  by cases x <;> simp [Std.Irrefl.irrefl]
+
+instance [LT α] [DecidableLT α] [Std.Irrefl (. < . : α → α → Prop)] : Std.Irrefl (. < . : (Option α) → (Option α) → Prop) where
+  irrefl := Option_lt_irrefl
+
+
+end CardanoLedgerApi.Extras
