Tests/Scripts.lean
@@ -1,5 +1,7 @@
 
+import Tests.Scripts.Governance.Properties
 import Tests.Scripts.HelloWorld.Properties
+import Tests.Scripts.MintingPolicy.Properties
 import Tests.Scripts.ParamFeed.Properties
 import Tests.Scripts.SellNFT.Properties
 import Tests.Scripts.UnlockPIN.Properties
