Tests/Scripts/Governance/Governance.lean
@@ -1,0 +1,14 @@
+import PlutusCore.UPLC
+import CardanoLedgerApi.V3
+
+namespace Tests.Scripts.Governance
+open CardanoLedgerApi.IsData.Class (toTerm)
+open CardanoLedgerApi.V3 (ScriptContext proposingInputs)
+open PlutusCore.ByteString (ByteString)
+open PlutusCore.UPLC.Term (Term)
+
+#import_uplc governance PlutusV3 single_cbor_hex "Tests/Scripts/Governance/governance.flat"
+
+#prep_uplc appliedGovernance governance proposingInputs 9000
+
+end Tests.Scripts.Governance
