Tests/Scripts/MintingPolicy/MintingPolicy.lean
@@ -1,0 +1,19 @@
+import PlutusCore.UPLC
+import CardanoLedgerApi.V3
+import Blaster
+
+namespace Tests.Scripts.MintingPolicy
+
+open CardanoLedgerApi.IsData.Class (toTerm)
+open CardanoLedgerApi.V3 (ScriptContext mintingInputs)
+open PlutusCore.ByteString (ByteString)
+open PlutusCore.UPLC.Term (Term)
+
+#import_uplc mintingPolicy PlutusV3 single_cbor_hex "Tests/Scripts/MintingPolicy/minting_policy.flat"
+
+def mintingPolicyInputs (paramsCs : ByteString) (ctx : ScriptContext) : List Term :=
+  toTerm paramsCs :: mintingInputs ctx
+
+#prep_uplc appliedMintingPolicy mintingPolicy mintingPolicyInputs 1200
+
+end Tests.Scripts.MintingPolicy
