Tests/Scripts/MintingPolicy/Properties.lean
@@ -1,0 +1,57 @@
+import CardanoLedgerApi.IsData.Class
+import CardanoLedgerApi.V3
+import Tests.Scripts.MintingPolicy.MintingPolicy
+import Blaster
+
+namespace Tests.Scripts.MintingPolicy
+open CardanoLedgerApi.IsData.Class
+open CardanoLedgerApi.V3
+open PlutusCore.UPLC.Utils
+open PlutusCore.ByteString (ByteString)
+open PlutusCore.Data (Data)
+
+set_option warn.sorry false
+
+def findMLogiScripHashInReferenceInputs (pparamsCs : ByteString) (inputs : List TxInInfo) : Option Credential :=
+  match inputs with
+  | [] => none
+  | x :: xs =>
+     if hasCurrencySymbol pparamsCs x.txInInfoResolved.txOutValue
+     then
+       match (txOutInlineDatum x.txInInfoResolved) with
+       | some (Data.Constr _ (Data.B bsh :: _)) => some (.ScriptCredential bsh)
+       | _ => none
+     else findMLogiScripHashInReferenceInputs pparamsCs xs
+
+def mintingLogicInWithdrawalMap (pparamsCs : ByteString) (ctx : ScriptContext) : Bool :=
+  match findMLogiScripHashInReferenceInputs pparamsCs ctx.scriptContextTxInfo.txInfoReferenceInputs with
+  | some cred => credentialInWithdrawals cred ctx.scriptContextTxInfo.txInfoWdrl
+  | none => False
+
+
+/-- Minting Policy successful → scriptInfo = minting logic is in withdrawal map -/
+theorem minting_policy_success_imp_mintScript_info_withdrawal :
+  ∀ (pparamsCs : ByteString) (ctx : ScriptContext),
+      validMintingContext ctx →
+      isSuccessful (appliedMintingPolicy.prop pparamsCs ctx) →
+      mintingLogicInWithdrawalMap pparamsCs ctx := by blaster
+
+/-- Minting logic not present in withdrawal map → Minting Policy must fail -/
+theorem logic_not_in_withdrawal_imp_minting_policy_fail :
+  ∀ (pparamsCs : ByteString) (ctx : ScriptContext),
+     validMintingContext ctx →
+     ¬ mintingLogicInWithdrawalMap pparamsCs ctx →
+     isUnsuccessful (appliedMintingPolicy.prop pparamsCs ctx) := by blaster
+
+/-- Counterexample expected if minting logic not in withdrawal map when minting policy is successful -/
+def minting_policy_success_imp_logic_not_in_withdrawal : Prop :=
+  ∀ (pparamsCs : ByteString) (ctx : ScriptContext),
+     validMintingContext ctx →
+     isSuccessful (appliedMintingPolicy.prop pparamsCs ctx) →
+     ¬ mintingLogicInWithdrawalMap pparamsCs ctx
+
+#blaster (gen-cex: 0) (solve-result: 1) [minting_policy_success_imp_logic_not_in_withdrawal]
+
+
+
+end Tests.Scripts.MintingPolicy
